cons ==> update

FreydSSA/Ctx/Var/Fun.lean
@@ -93,7 +93,7 @@ def FCtx.map_ty (Γ : FCtx ν α) (f : α → β) : FCtx ν β where
     generalize Γ.toFun x = a
     cases a <;> simp [WithTop.map, Top.top]
 
-def FCtx.cons (x : ν) (a : α) (Γ : FCtx ν α) : FCtx ν α where
+def FCtx.update (x : ν) (a : α) (Γ : FCtx ν α) : FCtx ν α where
   toFun := Function.update Γ.toFun x a
   support := Γ.support ∪ {x}
   mem_support_toFun := by
@@ -101,27 +101,27 @@ def FCtx.cons (x : ν) (a : α) (Γ : FCtx ν α) : FCtx ν α where
     simp only [Finset.mem_union, Function.update]
     split <;> simp [*, mem_support_toFun]
 
-theorem FCtx.cons_eq (x : ν) (y : ν) (a : α) (Γ : FCtx ν α)
-  (h : x = y) : (Γ.cons x a) y = a := by
-  simp [FCtx.cons, Function.update, DFunLike.coe, h]
+theorem FCtx.update_eq (x : ν) (y : ν) (a : α) (Γ : FCtx ν α)
+  (h : x = y) : (Γ.update x a) y = a := by
+  simp [FCtx.update, Function.update, DFunLike.coe, h]
 
-theorem FCtx.cons_app (x : ν) (a : α) (Γ : FCtx ν α) (y : ν)
-  : (Γ.cons x a) y = if y = x then ↑a else Γ y := by
-  simp [FCtx.cons, Function.update, DFunLike.coe]
+theorem FCtx.update_app (x : ν) (a : α) (Γ : FCtx ν α) (y : ν)
+  : (Γ.update x a) y = if y = x then ↑a else Γ y := by
+  simp [FCtx.update, Function.update, DFunLike.coe]
 
-theorem FCtx.cons_ne (x : ν) (a : α) (Γ : FCtx ν α) (y : ν)
+theorem FCtx.update_ne (x : ν) (a : α) (Γ : FCtx ν α) (y : ν)
   (h : y ≠ x)
-  : (Γ.cons x a) y = Γ y := by
-  simp [cons_app, h]
+  : (Γ.update x a) y = Γ y := by
+  simp [update_app, h]
 
-theorem FCtx.cons_mem_support_ne (x : ν) (a : α) (Γ : FCtx ν α)
-  (hx : y ≠ x) : y ∈ (Γ.cons x a).support → y ∈ Γ.support
-  := by simp [cons, hx]
+theorem FCtx.update_mem_support_ne (x : ν) (a : α) (Γ : FCtx ν α)
+  (hx : y ≠ x) : y ∈ (Γ.update x a).support → y ∈ Γ.support
+  := by simp [update, hx]
 
-def FCtx.cons_inj {x : ν} {a a' : α} {Γ : FCtx ν α}
-  (h : Γ.cons x a = Γ.cons x a') : a = a' :=
-  have hl : Γ.cons x a x = a := by simp [FCtx.cons, DFunLike.coe]
-  have hr : Γ.cons x a' x = a' := by simp [FCtx.cons, DFunLike.coe]
+def FCtx.update_inj {x : ν} {a a' : α} {Γ : FCtx ν α}
+  (h : Γ.update x a = Γ.update x a') : a = a' :=
+  have hl : Γ.update x a x = a := by simp [FCtx.update, DFunLike.coe]
+  have hr : Γ.update x a' x = a' := by simp [FCtx.update, DFunLike.coe]
   by rw [<-WithTop.coe_inj, <-hl, <-hr, h]
 
 def FCtx.get {Γ : FCtx ν α} (x : ν) (h : x ∈ Γ.support) : α :=
@@ -147,9 +147,9 @@ theorem FCtx.get_var {Γ : FCtx ν α} (x : ν) (a : α) (h : Γ x = a)
 theorem FCtx.get_eq_of {Γ Δ : FCtx ν α} {x y : ν} (hΓ : x ∈ Γ.support) (hΔ : y ∈ Δ.support) (h : Γ x = Δ y)
   : Γ.get x hΓ = Δ.get y hΔ := Option.some_injective _ $ ((Γ.get_eq hΓ).symm.trans h).trans (Δ.get_eq hΔ)
 
-theorem FCtx.cons_get_ne (x : ν) (a : α) (Γ : FCtx ν α) (hx : y ≠ x) (hy: y ∈ (Γ.cons x a).support)
-   : (Γ.cons x a).get y hy = Γ.get y (cons_mem_support_ne x a Γ hx hy)
-  := FCtx.get_eq_of hy (cons_mem_support_ne _ _ _ hx hy) (by simp [cons_app, hx])
+theorem FCtx.update_get_ne (x : ν) (a : α) (Γ : FCtx ν α) (hx : y ≠ x) (hy: y ∈ (Γ.update x a).support)
+   : (Γ.update x a).get y hy = Γ.get y (update_mem_support_ne x a Γ hx hy)
+  := FCtx.get_eq_of hy (update_mem_support_ne _ _ _ hx hy) (by simp [update_app, hx])
 
 def FCtx.Wk (Γ Δ : FCtx ν α) : Prop := ∀x, Δ x = ⊤ ∨ Δ x = Γ x
 
@@ -337,18 +337,18 @@ theorem FCtx.Wk.of_eq_on {Γ Δ : FCtx ν α}
 theorem FCtx.Wk.eq_on_iff {Γ Δ : FCtx ν α}
   : FCtx.Wk Γ Δ ↔ (∀x ∈ Δ.support, Δ x = Γ x) := ⟨eq_on, of_eq_on⟩
 
-theorem FCtx.Wk.cons {Γ Δ : FCtx ν α} (w : FCtx.Wk Γ Δ) (x : ν) (a : α)
-  : FCtx.Wk (Γ.cons x a) (Δ.cons x a) := by
+theorem FCtx.Wk.update {Γ Δ : FCtx ν α} (w : FCtx.Wk Γ Δ) (x : ν) (a : α)
+  : FCtx.Wk (Γ.update x a) (Δ.update x a) := by
   intro y
-  simp only [FCtx.cons, DFunLike.coe, Function.update]
+  simp only [FCtx.update, DFunLike.coe, Function.update]
   split
   simp
   exact w y
 
-theorem FCtx.Wk.cons_not_mem (x : ν) (a : α) (Γ : FCtx ν α) (hx : x ∉ Γ.support)
-  : FCtx.Wk (Γ.cons x a) Γ := by
+theorem FCtx.Wk.update_not_mem (x : ν) (a : α) (Γ : FCtx ν α) (hx : x ∉ Γ.support)
+  : FCtx.Wk (Γ.update x a) Γ := by
   intro y
-  simp only [cons_app]
+  simp only [update_app]
   split <;> simp [<-not_mem_support, *]
 
 theorem FCtx.Cmp.lsup_eq_rsup {Δ Δ' : FCtx ν α} (c : FCtx.Cmp Δ Δ')
