FreydSSA/Body/Fun/Basic.lean
@@ -6,16 +6,16 @@ variable {φ ν α} [Φ : InstSet φ (Ty α)]
 
 inductive UBody.FWf : Purity → FCtx ν (Ty α) → UBody φ ν → FCtx ν (Ty α) → Type _
   | nil (p) : Γ.Wk Δ → FWf p Γ nil Δ
-  | let1 (x) : e.FWf p Γ A → FWf p (Γ.cons x A) t Δ
+  | let1 (x) : e.FWf p Γ A → FWf p (Γ.update x A) t Δ
     → FWf p Γ (let1 x e t) Δ
   | let2 (x y) : e.FWf p Γ (Ty.pair A B) →
-    FWf p ((Γ.cons x A).cons y B) t Δ → FWf p Γ (let2 x y e t) Δ
+    FWf p ((Γ.update x A).update y B) t Δ → FWf p Γ (let2 x y e t) Δ
 
 def UBody.FWf.wkEntry {Γ' Γ Δ : FCtx ν (Ty α)} {t : UBody φ ν} (w: Γ'.Wk Γ)
   : FWf p Γ t Δ → FWf p Γ' t Δ
   | nil _ w' => nil _ (w.comp w')
-  | let1 x de dt => let1 x (de.wk w) (dt.wkEntry (w.cons x _))
-  | let2 x y de dt => let2 x y (de.wk w) (dt.wkEntry ((w.cons x _).cons y _))
+  | let1 x de dt => let1 x (de.wk w) (dt.wkEntry (w.update x _))
+  | let2 x y de dt => let2 x y (de.wk w) (dt.wkEntry ((w.update x _).update y _))
 
 def UBody.FWf.wkExit {Γ Δ Δ' : FCtx ν (Ty α)} {t : UBody φ ν} (dt : FWf p Γ t Δ) (w: Δ.Wk Δ')
   : FWf p Γ t Δ' := match dt with
@@ -51,10 +51,10 @@ theorem UBody.FWf.maxTrg_wk {Γ Δ : FCtx ν (Ty α)} {t : UBody φ ν} (dt : FW
 
 inductive UBody.FWfM : Purity → FCtx ν (Ty α) → UBody φ ν → FCtx ν (Ty α) → Type _
   | nil (p Γ) : FWfM p Γ nil Γ
-  | let1 (x) : e.FWf p Γ A → FWfM p (Γ.cons x A) t Δ
+  | let1 (x) : e.FWf p Γ A → FWfM p (Γ.update x A) t Δ
     → FWfM p Γ (let1 x e t) Δ
   | let2 (x y) : e.FWf p Γ (Ty.pair A B) →
-    FWfM p ((Γ.cons x A).cons y B) t Δ → FWfM p Γ (let2 x y e t) Δ
+    FWfM p ((Γ.update x A).update y B) t Δ → FWfM p Γ (let2 x y e t) Δ
 
 -- BUG: spurious unused variable warning
 set_option linter.unusedVariables false in
